Quantum_Separation_LogicDef.thy
@@ -4,31 +4,249 @@ begin
 
 type_synonym ('s,'p) triplet = "('s state) assn \<times> 'p \<times> ('s state) assn"
 
-context vars
-begin
+
+
 
 definition Q_domain_set::"'s expr_q \<Rightarrow> q_vars \<Rightarrow> 's expr_q "
   where "Q_domain_set q qvars \<equiv> (\<lambda>s. \<Union> (qvars ` q s))"
 
+
+
+
+definition comb_set::"('a \<Rightarrow> 'a \<Rightarrow> 'b) \<Rightarrow> 'a set \<Rightarrow> 'a set \<Rightarrow> 'b set"
+  where "comb_set f A B \<equiv> \<Union>a\<in>A. f a ` B " 
+
+
+lemma "a \<in> A \<Longrightarrow> b \<in> B \<Longrightarrow> f a b \<in> comb_set f A B"  
+  unfolding comb_set_def by auto
+
+lemma "x \<in> comb_set f A B \<Longrightarrow> \<exists>a b. a \<in> A \<and> b \<in> B \<and> x = f a b"  
+  unfolding comb_set_def by auto
+
+
 definition Q_sep_dis::"(('s state) \<Rightarrow> bool) \<Rightarrow> (('s state) \<Rightarrow> bool) \<Rightarrow>  (('s state) \<Rightarrow> bool)" 
 (infixr "\<and>*\<^sub>q" 35)
-where "Q_sep_dis A B \<equiv> (\<lambda>s. fst s \<in> (fst ` {s. A s \<and> B s}) \<and>  
-                            (fst (snd s) \<in> (fst ` (snd ` {s. A s \<and> B s}))) \<and>
-                            ((\<lambda>s. s \<in> (snd ` (snd ` {s. A s}))) \<and>* 
-                             (\<lambda>s. s \<in> (snd ` (snd ` {s. B s})))) (snd (snd s)))"
+where "Q_sep_dis A B \<equiv>  let setAB = fst ` (snd ` {s. A s}) \<inter>  fst ` (snd ` {s. B s});
+                              setA = {s. A s \<and> fst (snd s) \<in> setAB}; 
+                              setB = {s. B s \<and> fst (snd s) \<in> setAB} in
+                           (\<lambda>s. fst s \<in> (comb_set (*) (fst ` setA) (fst ` setB)) \<and>  
+                                 fst (snd s) \<in> setAB \<and>      
+                            ((\<lambda>s. s \<in> (snd ` (snd ` setA))) \<and>* 
+                             (\<lambda>s. s \<in> (snd ` (snd ` setB)))) (snd (snd s)))"
+
+definition stack\<^sub>s :: "('s state) set \<Rightarrow> 's set"
+  where "stack\<^sub>s A \<equiv> fst ` (snd ` A)"
+
+definition prob\<^sub>s :: "('s state) set \<Rightarrow> real set"
+  where "prob\<^sub>s A \<equiv> fst ` A"
+
+definition QState\<^sub>s :: "('s state) set \<Rightarrow> (complex) QStateM set"
+  where "QState\<^sub>s A \<equiv> snd ` (snd `  A)"
+
+
+definition eq_stack::"(('s state) set) \<Rightarrow> (('s state) set) \<Rightarrow> 's set"
+  where "eq_stack A B \<equiv> stack\<^sub>s A \<inter> stack\<^sub>s B"
+
+definition eq_stack_S::"(('s state) set) \<Rightarrow> 's set \<Rightarrow> (('s state) set) "
+  where "eq_stack_S A B \<equiv> {s. s \<in> A \<and> fst (snd s) \<in> B}"
+
+lemma eq_stacks_AB: "stack\<^sub>s (eq_stack_S A (eq_stack A B)) = stack\<^sub>s (eq_stack_S B (eq_stack A B))"
+  unfolding stack\<^sub>s_def eq_stack_S_def eq_stack_def
+  apply auto
+   apply (smt fst_conv image_iff mem_Collect_eq snd_conv)
+  by (smt fst_conv image_iff mem_Collect_eq snd_conv)
+  
+
+lemma eq_stack_stackS1: "get_stack (a,b,c) \<in> (eq_stack A B) \<Longrightarrow> get_stack (a,b,c) \<in> stack\<^sub>s (eq_stack_S A (eq_stack A B))" 
+  unfolding stack\<^sub>s_def eq_stack_S_def eq_stack_def
+  apply auto
+  by (smt fst_conv image_iff mem_Collect_eq snd_conv)
+
+lemma  eq_stack_stackS2: "get_stack (a,b,c) \<in> stack\<^sub>s (eq_stack_S A (eq_stack A B)) \<Longrightarrow> get_stack (a,b,c) \<in> (eq_stack A B)"
+  unfolding stack\<^sub>s_def eq_stack_S_def eq_stack_def
+  apply auto
+  by (smt fst_conv image_iff mem_Collect_eq snd_conv)
+
+lemma eq_stack_stack:"stack\<^sub>s (eq_stack_S A (eq_stack A B)) = eq_stack A B"
+  unfolding stack\<^sub>s_def eq_stack_S_def eq_stack_def
+  apply rule using eq_stack_stackS1 apply blast
+  using eq_stack_stackS2 by blast
+
+
+lemma stack_set_intro:
+  assumes a0:"(\<rho>a,\<sigma>,Q1) \<in> A" and a1:"(\<rho>b,\<sigma>,Q2) \<in> B"
+  shows "\<sigma>\<in> eq_stack A B "
+  using a0 a1 image_iff  unfolding eq_stack_def stack\<^sub>s_def by fastforce
+
+lemma comb_set_prob\<^sub>s_intro:
+  assumes 
+   a0:"(\<rho>a,\<sigma>,Q1) \<in> A" and
+   a1:"(\<rho>b,\<sigma>,Q2) \<in> B" 
+ shows  "\<rho>a*\<rho>b \<in> comb_set (*) (prob\<^sub>s  (eq_stack_S A (eq_stack A B))) (prob\<^sub>s (eq_stack_S B (eq_stack A B)))"
+proof-
+  have "(\<rho>a,\<sigma>,Q1) \<in> eq_stack_S A (eq_stack A B)"
+    unfolding eq_stack_S_def eq_stack_def stack\<^sub>s_def 
+    using a0 a1  image_iff by fastforce 
+  then have  "\<rho>a \<in> prob\<^sub>s  (eq_stack_S A (eq_stack A B))" 
+    using a0  unfolding prob\<^sub>s_def by (force simp add: image_iff)
+  moreover have "(\<rho>b,\<sigma>,Q2) \<in> eq_stack_S B (eq_stack A B)"
+    unfolding eq_stack_S_def eq_stack_def stack\<^sub>s_def 
+    using a0 a1  image_iff by fastforce
+  then have  "\<rho>b \<in> prob\<^sub>s  (eq_stack_S B (eq_stack A B))" 
+    using a1 unfolding prob\<^sub>s_def by (force simp add: image_iff)
+  ultimately show ?thesis unfolding comb_set_def
+    by blast
+qed     
+
+lemma quantu_set_QState\<^sub>s_intro:
+  assumes 
+   a0:"(\<rho>a,\<sigma>,Q1) \<in> A" and
+   a1:"(\<rho>b,\<sigma>,Q2) \<in> B" and
+   a2:"Q1 ## Q2" 
+ shows  "((\<lambda>s. s \<in> (QState\<^sub>s (eq_stack_S A (eq_stack A B)))) \<and>* 
+          (\<lambda>s. s \<in> (QState\<^sub>s (eq_stack_S B (eq_stack A B))))) (Q1 + Q2)"
+proof-
+  have "(\<rho>a,\<sigma>,Q1) \<in> eq_stack_S A (eq_stack A B)"
+    unfolding eq_stack_S_def eq_stack_def stack\<^sub>s_def 
+    using a0 a1  image_iff by fastforce 
+  then have  "Q1 \<in> QState\<^sub>s  (eq_stack_S A (eq_stack A B))" 
+    using a0  unfolding QState\<^sub>s_def by (force simp add: image_iff)
+  moreover have "(\<rho>b,\<sigma>,Q2) \<in> eq_stack_S B (eq_stack A B)"
+    unfolding eq_stack_S_def eq_stack_def stack\<^sub>s_def 
+    using a0 a1  image_iff by fastforce
+  then have  "Q2 \<in> QState\<^sub>s  (eq_stack_S B (eq_stack A B))" 
+    using a1 unfolding QState\<^sub>s_def by (force simp add: image_iff)
+  ultimately show ?thesis using a2 unfolding QState\<^sub>s_def unfolding sep_conj_def
+    by auto
+qed
+
+definition Q_sep_dis_set1::"(('s state) set) \<Rightarrow> (('s state) set) \<Rightarrow>  (('s state) set)" 
+(infixr "\<and>\<^sup>*1" 35)
+where "Q_sep_dis_set1 A B \<equiv>           
+         {(\<rho>,\<sigma>,Q). \<exists>\<rho>1 \<rho>2 Q1 Q2. (\<rho>1,\<sigma>,Q1) \<in> A \<and> (\<rho>2,\<sigma>,Q2) \<in> B \<and> 
+                   \<rho> = \<rho>1 * \<rho>2 \<and> Q1 ## Q2 \<and> Q = Q1 + Q2}" 
+
+definition Q_eq_stack_disj_heap::"(('s state) set) \<Rightarrow> (('s state) set) \<Rightarrow> ((('s state)\<times>('s state)) set)"
+  where "Q_eq_stack_disj_heap A B = 
+    {(a,b). a \<in> A \<and> b \<in> B \<and> get_stack a = get_stack b \<and>
+            (get_QStateM a)##(get_QStateM b)}"
 
 definition Q_sep_dis_set::"(('s state) set) \<Rightarrow> (('s state) set) \<Rightarrow>  (('s state) set)" 
 (infixr "\<and>\<^sup>*" 35)
-where "Q_sep_dis_set A B \<equiv> let eq_stack = (fst ` (snd ` A)) \<inter> (fst ` (snd ` B));
-                               eq_stack_S = (\<lambda>S. {s. s \<in> S \<and> fst (snd s) \<in> eq_stack})  in
-                            {s. \<forall>s1 s2. s1 \<in> eq_stack_S A \<and> s2 \<in> eq_stack_S B \<and> 
-                                   fst (snd s1) = fst (snd s2) \<longrightarrow> 
-                                fst s = fst s1 * fst s2 \<and> fst (snd s) = fst (snd s1) \<and>
-                               ((\<lambda>s. s \<in> (snd ` (snd ` {s. s = s1}))) \<and>* 
-                               (\<lambda>s. s \<in> (snd ` (snd ` {s. s = s2})))) (snd (snd s))}"
+where "Q_sep_dis_set A B \<equiv>  
+        (\<lambda>(a,b). (get_prob a * get_prob b, (get_stack a, get_QStateM a + get_QStateM b))) ` 
+       Q_eq_stack_disj_heap A B" 
+
+lemma eq_qsep1:"x \<in> (xa \<and>\<^sup>*1 xb) \<Longrightarrow> x \<in> (xa \<and>\<^sup>* xb)"
+  unfolding Q_sep_dis_set_def Q_sep_dis_set1_def Let_def get_stack_def get_prob_def get_QStateM_def
+            image_def Q_eq_stack_disj_heap_def
+  apply (auto simp add: case_prod_beta)   
+    by (metis prod.collapse)
+  
+
+lemma eq_qsep2:"xb \<in> (x \<and>\<^sup>* xa) \<Longrightarrow> xb \<in> (x \<and>\<^sup>*1 xa)"
+  unfolding Q_sep_dis_set_def Q_sep_dis_set1_def Let_def get_stack_def get_prob_def get_QStateM_def
+            image_def Q_eq_stack_disj_heap_def  
+  by auto
+  
+
+lemma eq_Qsep_dis_sets:"Q_sep_dis_set1 =  Q_sep_dis_set"
+  apply rule   
+  apply rule 
+  apply rule 
+   apply rule 
+   apply (rule eq_qsep1, simp)
+  apply (rule)
+  by (rule eq_qsep2, simp)
+
+  
+lemma Q_sep_dis_set_empty1:
+  assumes  a0:"Q_eq_stack_disj_heap A B = {}"
+         shows "Q_sep_dis_set A B = {}"
+  using a0 
+  unfolding Q_sep_dis_set_def 
+  by auto
+
+
+lemma Q_sep_dis_set_empty2:
+  assumes  a0:"Q_sep_dis_set A B = {}" 
+  shows "Q_eq_stack_disj_heap A B = {}"
+  using a0 
+  unfolding Q_sep_dis_set_def 
+  by auto
+
+lemma h0: assumes a0:"fst ` snd ` A \<inter> fst ` snd ` B \<noteq> {}"
+  shows "\<exists>a aa.
+       \<exists>ab\<in>B.
+          fst (snd ab) \<in> fst ` snd ` A \<and>
+          (\<exists>b. (aa, fst (snd ab), b) \<in> A) \<and>
+          a \<in> (*) aa ` fst ` {s \<in> B. fst (snd s) \<in> fst ` snd ` A \<and> fst (snd s) \<in> fst ` snd ` B}"
+proof-
+  obtain aa ab x ba bb where 
+      a1:"x\<in>fst ` snd ` A" and a2:"x\<in>fst ` snd ` B" and a3:"(aa,x,ab)\<in>A" and a4:"(ba,x,bb)\<in>B" 
+    using a0 apply auto
+    by (metis (no_types) fst_conv image_iff snd_conv)   
+  then show ?thesis
+    apply auto using a1 a2 a3 a4
+    by (smt all_not_in_conv fst_conv image_is_empty mem_Collect_eq snd_conv)
+qed      
+
+lemma h1: assumes a0:"eq_stack A B \<noteq> {}"
+  shows "\<exists>a aa.
+       \<exists>ab\<in>A.
+          fst (snd ab) \<in> fst ` snd ` B \<and>
+          (\<exists>b. (aa, fst (snd ab), b) \<in> A) \<and>
+          a \<in> (*) aa ` fst ` {s \<in> B. fst (snd s) \<in> fst ` snd ` A \<and> fst (snd s) \<in> fst ` snd ` B}"
+proof-
+  obtain aa ab x ba bb where 
+      a1:"x\<in>fst ` snd ` A" and a2:"x\<in>fst ` snd ` B" and a3:"(aa,x,ab)\<in>A" and a4:"(ba,x,bb)\<in>B" 
+    using a0 unfolding eq_stack_def stack\<^sub>s_def apply auto
+    by (metis (no_types) fst_conv image_iff snd_conv)   
+  then show ?thesis
+    apply auto using a1 a2 a3 a4
+    by (smt all_not_in_conv fst_conv image_is_empty mem_Collect_eq snd_conv)
+qed      
+
+
+lemma Q_sep_dis_set_dest:
+  assumes a0:"(\<rho>, \<sigma>, Q) \<in> (A \<and>\<^sup>* B)"
+  shows "\<exists>\<rho>1 \<rho>2 Q1 Q2. \<rho> = \<rho>1 * \<rho>2 \<and> 
+           (\<rho>1, \<sigma>, Q1) \<in> A \<and> (\<rho>2, \<sigma>, Q2) \<in> B \<and> 
+            Q =  Q1 + Q2 \<and> Q1 ## Q2"
+  using a0  
+  apply (auto simp add: eq_Qsep_dis_sets[THEN sym])
+  unfolding Q_sep_dis_set1_def
+  by auto     
+
+lemma Q_sep_dis_set_elim:
+  "(\<rho>, \<sigma>, Q) \<in> (A \<and>\<^sup>* B) \<Longrightarrow>
+    \<lbrakk>\<And>\<rho>1 \<rho>2 Q1 Q2. \<rho> = \<rho>1 * \<rho>2 \<and> 
+           (\<rho>1, \<sigma>, Q1) \<in> A \<and> (\<rho>2, \<sigma>, Q2) \<in> B \<and> 
+            Q =  Q1 + Q2 \<and> Q1 ## Q2 \<Longrightarrow> P\<rbrakk> \<Longrightarrow>
+    P" 
+  by (auto dest:  Q_sep_dis_set_dest)
+
+lemma Q_sep_dis_set_intro:
+ assumes 
+   a0:"(\<rho>a,\<sigma>,Q1) \<in> A" and
+   a1:"(\<rho>b,\<sigma>,Q2) \<in> B" and
+   a2:"Q1 ## Q2" 
+ shows "(\<rho>a*\<rho>b, \<sigma>, Q1 + Q2) \<in> Q_sep_dis_set A B"   
+  using a1 a2 a0
+  unfolding Q_sep_dis_set_def get_prob_def get_stack_def get_QStateM_def Let_def
+            eq_stack_def comb_set_def stack\<^sub>s_def prob\<^sub>s_def eq_stack_S_def QState\<^sub>s_def
+  image_def Q_eq_stack_disj_heap_def
+  apply (auto simp add: case_prod_beta)
+  by blast
+
+
 \<comment>\<open>map_assn' receives two sets of qbits q1 q2 addresses and a vector v. It represents that the current
   qstate is equal to v and that v can be split into two different separated qstates each
  of them is composed by the qubits contained by the sets q1 and q2\<close>
+  
+  
+     
+  
 (*definition map_assn'::"'s expr_q \<Rightarrow> 's expr_q \<Rightarrow> ('s state, (complex) QState) expr \<Rightarrow> (('s state) set)"  
  ("_\<cdot>_ \<mapsto> _"  [1000, 20, 1000] 60)
   where "map_assn' q1 q2 v \<equiv> let qs = (\<lambda>s. snd (get_qstate s));
@@ -77,24 +295,96 @@ definition map_assn'::"'s expr_q \<Rightarrow> 's expr_q \<Rightarrow> ('s, (com
   It represents that the current qstate is v and that it can be split into two different separated qstates
   and the set of qubits of one of them is the set of qubits in q1\<close>
 
-definition map_assnl::"('s,nat set) expr \<Rightarrow> ('s, (complex) QState) expr \<Rightarrow> (('s state) set)"  (infixr "\<mapsto>\<^sub>l" 35)
+(* definition map_assnl::"('s,nat set) expr \<Rightarrow> ('s, (complex) QState) expr \<Rightarrow> (('s state) set)"  (infixr "\<mapsto>\<^sub>l" 35)
   where "map_assnl f v \<equiv> let qv = (\<lambda>s. fst (get_qstate s)); 
                             qs = (\<lambda>s. snd (get_qstate s));
                             st = (\<lambda>s. get_stack s) in   
                  {s. Q_domain_set f (qv s) (st s) \<noteq> {} \<and> Q_domain_set f (qv s) (st s) = QState_vars (v (st s)) \<and>
-                     (\<exists>\<qq>' \<qq>''. (qs s) =  \<qq>' + \<qq>'' \<and> (v (st s)) = \<qq>''  \<and> \<qq>' ## \<qq>'' )}"
+                     (\<exists>\<qq>' \<qq>''. (qs s) =  \<qq>' + \<qq>'' \<and> (v (st s)) = \<qq>''  \<and> \<qq>' ## \<qq>'' )}" *)
 
-definition map_assnla::"('s,nat set) expr \<Rightarrow> ('s, (complex) list) expr \<Rightarrow> (('s state) set)"
-(infixr "1\<mapsto>\<^sub>l" 35)
-  where "map_assnla f v \<equiv> let qv = (\<lambda>s. fst (get_qstate s)); 
+context vars 
+begin
+
+definition map_assnl::"('s,nat set) expr \<Rightarrow> ('s, (complex) list) expr \<Rightarrow> (('s state) set)"
+(infixr "\<mapsto>\<^sub>l" 40)
+  where "map_assnl f v \<equiv> let qv = (\<lambda>s. fst (get_qstate s)); 
                             qs = (\<lambda>s. snd (get_qstate s));
                             st = (\<lambda>s. get_stack s) in   
-                 {s. Q_domain_set f (qv s) (st s) \<noteq> {} \<and> 
-                     (\<exists>\<qq>' \<qq>''. (qs s) =  \<qq>' + \<qq>'' \<and> \<qq>' ## \<qq>'' \<and>  
+                 {s. (\<exists>\<qq>' \<qq>''. (qs s) =  \<qq>' + \<qq>'' \<and> \<qq>' ## \<qq>'' \<and>  
                                 QState_vars \<qq>'' = Q_domain_set f (qv s) (st s) \<and>
                                QState_list \<qq>'' = (v (st s)))}"
 
- 
+definition map_assn::"('s,nat set) expr \<Rightarrow> ('s, (complex) list) expr \<Rightarrow> (('s state) set)"
+(infixr "\<mapsto>" 40)
+  where "map_assn f v \<equiv> let qv = (\<lambda>s. fst (get_qstate s)); 
+                            qs = (\<lambda>s. snd (get_qstate s));
+                            st = (\<lambda>s. get_stack s) in   
+                 {s. QState_vars (qs s)  = Q_domain_set f (qv s) (st s) \<and>
+                     QState_list (qs s) = (v (st s))}"
+
+
+definition map_assnv1::"'v  \<Rightarrow> ('s, (complex) list) expr \<Rightarrow> (('s state) set)"
+(infixr "\<mapsto>\<^sub>v" 40)
+  where "map_assnv1 v q \<equiv> let qv = (\<lambda>s. fst (get_qstate s)); 
+                            qs = (\<lambda>s. snd (get_qstate s));
+                            st = (\<lambda>s. get_stack s);
+                            set_v = (\<lambda>st. {to_nat (get_value st v )}) in   
+                 {s. QState_vars (qs s)  = Q_domain_var (set_v (st s)) (qv s) \<and>
+                     QState_list (qs s) = (q (st s))}" 
+
+definition map_assnv::"'v  \<Rightarrow> ('s, nat set) expr \<Rightarrow> ('s, (complex) list) expr \<Rightarrow> (('s state) set)"
+("_\<cdot>_ \<mapsto>\<^sub>v _" [1000, 20, 1000] 60)
+  where "map_assnv v i q \<equiv> let qv = (\<lambda>s. fst (get_qstate s)); 
+                            qs = (\<lambda>s. snd (get_qstate s));
+                            st = (\<lambda>s. get_stack s);
+                            set_v = (\<lambda>st. var_set v i st) in   
+                 {s. QState_vars (qs s)  = Q_domain_var (set_v (st s)) (qv s) \<and>
+                     QState_list (qs s) = (q (st s))}"
+
+definition prob_assert::" (('s state) set) \<Rightarrow>  real \<Rightarrow> (('s state) set)"
+(infixr "\<smile>" 60)
+  where "prob_assert q p \<equiv> {s. fst s = p \<and> snd s \<in> {(x,y). \<exists>p. (p,(x,y)) \<in> q}} "
+
+definition int_stack_ass::"('s,'a set) expr \<Rightarrow> ('s, 'a set) expr \<Rightarrow> (('s state) set)"
+(infixr "\<inter>\<^sub>{\<^sub>}" 35)
+  where "int_stack_ass q1 q2 \<equiv> let st = (\<lambda>s. get_stack s) in   
+                 {s. q1 (st s) \<inter> q2 (st s) = {}}"
+
+(* definition empty_state_norm_expr::"('s, complex) expr \<Rightarrow> ('s , complex QState) expr"
+("|>\<^sub>_" 50)
+where "empty_state_norm_expr n \<equiv> (\<lambda>s. (n s) \<cdot>\<^sub>q |>)" *)
+
+definition empty_qstatem_norm_expr::"('s, complex) expr \<Rightarrow> ('s , complex QStateM) expr"
+("|>\<^sub>_" 50)
+where "empty_qstatem_norm_expr n \<equiv> (\<lambda>s. QStateM ({}\<^sub>q, (n s) \<cdot>\<^sub>q |>))"
+
+
+definition empty_qstatem_norm_ass::"('s, complex) expr \<Rightarrow> (('s state) set)"
+("/|>a\<^sub>_" 50)
+where "empty_qstatem_norm_ass n \<equiv> let h = |>\<^sub>n in 
+                                 {s. get_QStateM s = (h (get_stack s))}"
+
+
+definition Q_sep_dis_q::"(('s state) set) \<Rightarrow> (('s state) set) \<Rightarrow>  (('s state) set)" 
+(infixr "\<and>\<^sub>q" 35)
+where "Q_sep_dis_q q1 q2 \<equiv> {s. ((\<lambda>s. s \<in> (snd ` (snd ` q1))) \<and>* 
+                                (\<lambda>s. s \<in> (snd ` (snd ` q2)))) (snd (snd s))}"
+
+definition QState_expr::"('s , nat set) expr \<Rightarrow> ('s, complex list) expr \<Rightarrow> ('s,complex QState) expr"
+  where "QState_expr v l \<equiv>  (\<lambda>s. QState (v s, l s))"
+
+definition QState_plus_expr::"('s,complex QState) expr \<Rightarrow> ('s,complex QState) expr \<Rightarrow> ('s,complex QState) expr"
+(infixr "+\<^sub>e" 50)
+  where "QState_plus_expr q1 q2 \<equiv> (\<lambda>s. (q1 s) + (q2 s))"
+
+definition QStateM_expr::"('s,complex QState) expr \<Rightarrow> ('s state, complex QStateM) expr"
+where "QStateM_expr q1 \<equiv> let qv = (\<lambda>s. fst (get_qstate s)); 
+                            qs = (\<lambda>s. snd (get_qstate s));
+                            st = (\<lambda>s. get_stack s);
+                            f = (\<lambda>S qv s. if s \<in> S then qv s else {}) in
+                          (\<lambda>s. QStateM(f (QState_vars (qs s)) (qv s), q1 (st s)))"
+
+
 
 (* definition map_assnl::"('s,nat set) expr \<Rightarrow> ('s state, (complex) QState) expr \<Rightarrow> (('s state) set)"  (infixr "\<mapsto>\<^sub>l" 35)
   where "map_assnl f v \<equiv> let qv = (\<lambda>s. fst (get_qstate s)); 
@@ -133,18 +423,35 @@ definition aij::"'s expr_q \<Rightarrow> q_vars \<Rightarrow> ('s, (complex) QSt
 
 definition v_f::"'s expr_q \<Rightarrow> q_vars \<Rightarrow> ( nat \<Rightarrow>'s  \<Rightarrow>  complex) \<Rightarrow> ('s, (complex) QState) expr"
   where "v_f q qvars f \<equiv> let vars = Q_domain_set q qvars in 
-                     (\<lambda>s. QState(vars s, 
-                          map (\<lambda>e. f e s) [0..<2^card (vars s)]))"
+                     (\<lambda>s. QState(vars s, map (\<lambda>e. f e s) [0..<2^card (vars s)]))"
+
 
 definition var_exp::"'v \<Rightarrow> 's \<Rightarrow> nat set"
 ("\<llangle>_\<rrangle>"  [] 1000)
-  where "var_exp q  \<equiv> \<lambda>\<sigma>. {to_nat (get_value \<sigma> q)}"
+where "var_exp q  \<equiv> \<lambda>\<sigma>. {to_nat (get_value \<sigma> q)}"
+
+
 
 definition valid::"[('s state) assn,('v, 's) com,('s state) assn] \<Rightarrow> bool"
     ("\<Turnstile>_ _ _"  [1000, 20, 1000] 60)
     where "\<Turnstile> P c Q \<equiv> \<forall>\<sigma> \<sigma>'. \<turnstile> \<langle>c,\<sigma>\<rangle> \<Rightarrow> \<sigma>' \<longrightarrow> \<sigma> \<in> Normal ` P \<longrightarrow> \<sigma>' \<noteq> Fault \<longrightarrow>
                             \<sigma>' \<in> Normal ` Q"
 
+definition \<SS>::"('s state) set \<Rightarrow> ('s \<Rightarrow> real \<Rightarrow> complex QStateM \<Rightarrow> bool)"
+  where "\<SS> s \<equiv> (\<lambda>u p q. (p,u,q) \<in> s)"
+
+
+lemma \<SS>_equiv:"s \<in> R \<longleftrightarrow> (\<SS> R) (get_stack s)  (get_prob s) (get_QStateM s)" 
+  unfolding  \<SS>_def get_stack_def get_prob_def get_QStateM_def by auto
+
+lemma allocate_preserves_R:
+  assumes a2':"\<sigma>' = set_value \<sigma> q (from_nat q')" and       
+       a6:"not_access_v (\<SS> R) q" and a7:"q \<in> variables" and  a8:"q \<in> nat_vars" and
+       a9:"(p,\<sigma>,\<Q>) \<in> R"
+     shows "(p,\<sigma>',\<Q>) \<in> R"   
+  using not_access_v_f_q_eq_set[OF a7 from_nat_in_vdomain[OF a7 a8] a2' a6] assms 
+  unfolding \<SS>_equiv get_stack_def get_prob_def get_QStateM_def
+  by auto
 
 inductive "hoarep"::"[('s state) assn,('v,'s) com, ('s state) assn] => bool"
     ("\<turnstile>(_/ (_)/ _)" [1000,20,1000]60)
@@ -187,22 +494,24 @@ where
                  (set_stack s (set_value (st s) q (from_nat (the_elem ((\<llangle>q\<rrangle>) (st s)))))) \<in> ((\<llangle>q\<rrangle>) \<mapsto>\<^sub>l Qs)}
               (Alloc q e v) (\<llangle>q\<rrangle> \<mapsto>\<^sub>l Qs)"
 *)
-| QAlloc:"not_access_v v q \<Longrightarrow>          
-          q \<in> variables \<Longrightarrow> is_nat q \<Longrightarrow>
-          \<turnstile> {s. True }  (Alloc q e v) (\<llangle>q\<rrangle> 1\<mapsto>\<^sub>l v)"
+| QAlloc:"not_access_v v q \<Longrightarrow> not_access_v (\<SS> R) q \<Longrightarrow>         
+          q \<in> variables \<Longrightarrow> q \<in> nat_vars \<Longrightarrow>
+          \<turnstile> R q:=alloc[e] v ((q\<cdot>f \<mapsto>\<^sub>v v) \<smile> 1 \<and>\<^sup>* R)"
 
 
 \<comment>\<open>In QDispose we set that Qs does not depend on the stack to avoid that 
    the n in the postcondition may also depend on the stack and gives unsound results
   in later modifications to the stack that may not affect the vector\<close>
-| QDispose: "qv = (\<lambda>s. fst (get_qstate s)) \<and> st =(\<lambda>s. get_stack s) \<Longrightarrow> not_access_v n q \<Longrightarrow>               
-             n = (\<lambda>s. vec_norm (QState_vector (Qs s))) \<Longrightarrow>
-             P = ((\<llangle>q\<rrangle> \<mapsto>\<^sub>l Qs) \<inter> (q1 \<mapsto>\<^sub>l Qs') \<inter>  
-              {s. (get_qstate s) = s1 + s2 \<and> 
-                  Q_domain (fst s1) = Q_domain_set \<llangle>q\<rrangle> (qv s) (st s) \<and> 
-                  Q_domain (fst s2) = Q_domain_set q1 (qv s) (st s) \<and>
-                  set_qstate s (QStateM(fst s2 ,snd s2+ (n (st s)) \<cdot>\<^sub>q |>)) \<in>Q}) \<Longrightarrow> 
-              \<turnstile> P (Dispose q) Q" 
+(* | QDispose: "not_access_v n q \<Longrightarrow>               
+             n = (\<lambda>s. vec_norm (vec_of_list (v1 s))) \<Longrightarrow>
+             P = (\<llangle>q\<rrangle> \<mapsto>\<^sub>l v1) \<inter> (q1 \<mapsto>\<^sub>l v2) \<inter> (\<llangle>q\<rrangle> \<inter>\<^sub>{\<^sub>} q1) \<inter>
+             {s. set_qstate s 
+                 ((QStateM_expr ((QState_expr q1 v2) +\<^sub>e |>\<^sub>n)) s) \<in> Q} \<Longrightarrow> 
+              \<turnstile> P (Dispose q) Q"  *)
+
+ | QDispose: "q \<in> variables \<Longrightarrow> q \<in> nat_vars \<or> q \<in> nat_list_vars  \<Longrightarrow>            
+               n = (\<lambda>s. vec_norm (vec_of_list (v s))) \<Longrightarrow>                  
+              \<turnstile> ((q\<cdot>i \<mapsto>\<^sub>v v) \<and>\<^sup>* R) (Dispose q i) (( |>a\<^sub>n) \<and>\<^sup>* R)"  
 
 (* | QMeasure1: " \<turnstile> {s.  \<exists>k. pr = get_prob s \<and> qv = fst (get_qstate s) \<and> qs = snd (get_qstate s) \<and> st = get_stack s \<and> 
                  q (st, qv) \<subseteq> (QState_vars qs) \<and> 
@@ -240,10 +549,127 @@ where
            \<Longrightarrow> \<turnstile> P c Q"
 
 
+  
+lemma prob_assert_dest:"s \<in> P \<smile> 1 \<Longrightarrow> get_prob s = 1 \<and> (\<exists>s'. (s',snd s) \<in> P)"
+  unfolding prob_assert_def get_prob_def by auto
+
+
+(* lemma map_assnv_prob:
+   "QState_wf (q'_addr, v \<sigma>) \<Longrightarrow> QStateM_wf ((\<lambda>i. {})(q' := q'_addr), QState (q'_addr, v \<sigma>)) \<Longrightarrow> 
+       QStateM_map (QStateM ((\<lambda>i. {})(q' := q'_addr), QState (q'_addr, v \<sigma>))) = (\<lambda>i. {})(q' := q'_addr) \<Longrightarrow>
+        length (v \<sigma>) = 2^e \<sigma> \<Longrightarrow>  
+      length (v (set_value \<sigma> q (from_nat q'))) = 2^e \<sigma> \<Longrightarrow> q \<in> variables \<Longrightarrow>
+     v \<sigma> = v (set_value \<sigma> q (from_nat q')) \<Longrightarrow>
+      (1, set_value \<sigma> q (from_nat q'),
+         QStateM ((\<lambda>i. {})(q' := q'_addr), QState (q'_addr, v \<sigma>)))
+           \<in> (q \<mapsto>\<^sub>v v) \<smile> 1"
+ unfolding prob_assert_def map_assnv_def Let_def get_qstate_def get_stack_def Q_domain_var_def set_value_def
+  apply auto        
+     apply (metis QStateM_rel1 QState_var_idem  fst_conv snd_conv)
+  using QStateM_rel1 QState_var_idem  apply fastforce 
+    apply (metis QStateM_rel2 QStateM_wf_qstate QState_list_idem  fst_conv snd_conv )      
+  apply (simp add:  get_set rep_nat set_value_def)
+  by (simp add:  get_set rep_nat) *)
+
+lemma map_assnv_prob:
+   "QState_wf (q'_addr, v \<sigma>) \<Longrightarrow> QStateM_wf ((\<lambda>i. {})(q' := q'_addr), QState (q'_addr, v \<sigma>)) \<Longrightarrow> 
+       QStateM_map (QStateM ((\<lambda>i. {})(q' := q'_addr), QState (q'_addr, v \<sigma>))) = (\<lambda>i. {})(q' := q'_addr) \<Longrightarrow>
+        length (v \<sigma>) = 2^e \<sigma> \<Longrightarrow> q \<in> nat_vars  \<Longrightarrow> 
+      length (v (set_value \<sigma> q (from_nat q'))) = 2^e \<sigma> \<Longrightarrow> q \<in> variables \<Longrightarrow>
+     v \<sigma> = v (set_value \<sigma> q (from_nat q')) \<Longrightarrow>
+      (1, set_value \<sigma> q (from_nat q'),
+         QStateM ((\<lambda>i. {})(q' := q'_addr), QState (q'_addr, v \<sigma>)))
+           \<in> (q\<cdot>f \<mapsto>\<^sub>v v) \<smile> 1"
+  unfolding prob_assert_def map_assnv_def Let_def get_qstate_def get_stack_def 
+            Q_domain_var_def set_value_def var_set_def
+  apply auto
+  apply (simp add: get_set rep_nat)
+     apply (metis QStateM_rel1 QState_var_idem  fst_conv snd_conv)
+  using QStateM_rel1 QState_var_idem  apply fastforce 
+    apply (metis QStateM_rel2 QStateM_wf_qstate QState_list_idem  fst_conv snd_conv )      
+  apply (simp add:  get_set rep_nat set_value_def)
+  by (simp add:  get_set rep_nat )
+
+
 lemma alloc_sound:
+  assumes (* a0: "st =(\<lambda>s. get_stack s) " and *) a1:"not_access_v v q" and 
+          a2':"not_access_v (\<SS> R) q" and 
+          a3:"q \<in> variables" and  a4:"q \<in> nat_vars"
+  shows "\<Turnstile> R q:=alloc[e] v (( (q\<cdot>f \<mapsto>\<^sub>v v)) \<smile> 1 \<and>\<^sup>* R)"  
+proof-
+  { fix s s'
+    let ?st = "(\<lambda>s. get_stack s) "
+     assume a00:"\<turnstile> \<langle>q:=alloc[e] v,s\<rangle> \<Rightarrow> s'" and
+            a01:"s \<in> Normal ` R" and
+            a02:"s' \<noteq> Fault"
+     then obtain sn where a01:"s = Normal sn" and         
+         a01a:"sn \<in> R"  
+       by auto               
+     then obtain q' \<Q> q'_addr \<sigma> \<delta> where 
+      sn: "sn = (\<delta>, \<sigma>, \<Q>)" and 
+      s':"s' = Normal (\<delta>, set_value \<sigma> q (from_nat q'),
+                         \<Q> + QStateM ((\<lambda>i. {})(q' := q'_addr), QState (q'_addr, v \<sigma>)))" and
+      q':"q' \<notin> dom_q_vars (QStateM_map \<Q>)" and
+      q'_addr_in_new: "q'_addr \<in> new_q_addr e \<sigma> (QStateM_map \<Q>)" and 
+      e_gt0:"0 < e \<sigma>" and e_eq_v:"length (v \<sigma>) = 2^e \<sigma>" 
+        using  a02
+        by (auto intro: QExec_Normal_elim_cases(9)[OF a00[simplified a01]])    
+    then obtain sn' where 
+       sn':"s' = Normal sn' \<and> 
+        sn' = (\<delta>, set_value \<sigma> q (from_nat q'), \<Q> + QStateM ((\<lambda>i. {})(q' := q'_addr), QState (q'_addr, v \<sigma>)))" 
+       by auto              
+     let ?\<Q> = "\<Q> + QStateM ((\<lambda>i. {})(q' := q'_addr), QState (q'_addr, v \<sigma>))" 
+     have \<sigma>:"\<sigma> = ?st sn" and Q:"QStateM_unfold \<Q> = get_qstate sn" and 
+          Q':"QStateM_unfold ?\<Q> = get_qstate sn'"
+       using sn  sn' unfolding get_qstate_def get_stack_def   by auto
+     let ?\<sigma>' = "set_value \<sigma> q (from_nat q')" 
+     let ?\<Q>' = "QStateM ((\<lambda>i. {})(q' := q'_addr), QState (q'_addr, v \<sigma>))"   
+     
+     have st':"?st sn' = ?\<sigma>'" using sn' unfolding get_stack_def   
+       by auto     
+     have v_eq:"v \<sigma> = v ?\<sigma>'" 
+       by (metis a3 a4 from_nat_in_vdomain local.a1 not_access_v_f_q_eq_set st')
+     then  have e_eq_v':"length (v ?\<sigma>') = 2^e \<sigma>"
+       using e_eq_v by auto
+     have q'_addr:"(q'_addr) \<noteq> {}" using e_gt0 q'_addr_in_new 
+       unfolding new_q_addr_def by auto    
+     have sn_mod_\<sigma>'_in_R:"(\<delta>, ?\<sigma>', \<Q>) \<in> R" using a01a st' unfolding get_stack_def
+       using a2' a3 a4 allocate_preserves_R sn by blast
+     have new_state_in_assr:"(1, ?\<sigma>', ?\<Q>') \<in> (q\<cdot>f \<mapsto>\<^sub>v v) \<smile> 1"
+       using map_assnv_prob[OF _ _ _ ] e_eq_v e_eq_v'  v_eq a4
+          allocate_wf1[of ?\<Q>', OF _  _ _ q'_addr_in_new e_gt0, of  "(\<lambda>i. {})(q' := q'_addr)" v q' ?\<sigma>' set_value q, simplified, OF e_eq_v]
+       by (simp add: a3)
+     have "sn' \<in> ((q\<cdot>f \<mapsto>\<^sub>v v) \<smile> 1 \<and>\<^sup>* R)"       
+     proof-    
+       let ?A = "(q\<cdot>f \<mapsto>\<^sub>v v) \<smile> 1" and ?B = R
+       let ?A' = "eq_stack_S ?A (eq_stack ?A ?B)"
+       let ?B' = "eq_stack_S ?B (eq_stack ?A ?B)"       
+       have "get_prob sn' \<in> (comb_set (*) (prob\<^sub>s  ?A') (prob\<^sub>s  ?B'))"
+         using prob_assert_dest comb_set_prob\<^sub>s_intro[OF new_state_in_assr sn_mod_\<sigma>'_in_R] sn'              
+         unfolding get_prob_def by auto
+       moreover have "get_stack sn' \<in> eq_stack ?A ?B"
+         using stack_set_intro[OF new_state_in_assr sn_mod_\<sigma>'_in_R]
+         by (simp add: st')
+       moreover have h:"QStateM ((\<lambda>i. {})(q' := q'_addr), QState (q'_addr, v \<sigma>)) ## \<Q>"
+         using disjoint_allocate[of ?\<Q>', OF _ q' _ _ q'_addr_in_new e_gt0, of "(\<lambda>i. {})(q' := q'_addr)" v ?\<sigma>' set_value q, simplified, OF e_eq_v]         
+         using sep_disj_commuteI by blast 
+       then have "((\<lambda>s. s \<in> (QState\<^sub>s ?A')) \<and>* (\<lambda>s. s \<in> (QState\<^sub>s  ?B'))) (get_QStateM sn')"
+         using quantu_set_QState\<^sub>s_intro[OF new_state_in_assr sn_mod_\<sigma>'_in_R] sn' 
+         unfolding get_QStateM_def
+         by (simp add: sep_add_commute)
+       show ?thesis 
+         using Q_sep_dis_set_intro[OF new_state_in_assr sn_mod_\<sigma>'_in_R h]         
+         unfolding get_prob_def comb_set_def get_stack_def
+         by (simp add: local.h sep_add_commute sn')
+     qed
+    then have "s' \<in> Normal ` ((q\<cdot>f \<mapsto>\<^sub>v v) \<smile> 1 \<and>\<^sup>* R)" using sn' by auto  
+   } thus ?thesis unfolding valid_def by auto
+ qed
+
+(* lemma alloc_sound:
   assumes (* a0: "st =(\<lambda>s. get_stack s) " and *) a1:"not_access_v v q" and
           a3:"q \<in> variables" and  a4:"is_nat q"
-  shows "\<Turnstile>{s. True } q:=alloc[e] v (\<llangle>q\<rrangle> 1\<mapsto>\<^sub>l v)"  
+  shows "\<Turnstile>{s. True } q:=alloc[e] v (\<llangle>q\<rrangle> \<mapsto>\<^sub>l v)"  
 proof-
   { fix s s'
     let ?st = "(\<lambda>s. get_stack s) "
@@ -270,19 +696,18 @@ proof-
      let ?\<Q> = "\<Q> + QStateM ((\<lambda>i. {})(q' := q'_addr), QState (q'_addr, v \<sigma>))" 
      have \<sigma>:"\<sigma> = ?st sn" and Q:"QStateM_unfold \<Q> = get_qstate sn" and 
           Q':"QStateM_unfold ?\<Q> = get_qstate sn'"
-       using sn  sn' unfolding get_stack_def get_qstate_def by auto
+        unfolding get_stack_def  get_qstate_def using sn  sn' by auto
      let ?\<sigma>' = "set_value \<sigma> q (from_nat q')" 
-     let ?\<Q>' = "QStateM ((\<lambda>i. {})(q' := q'_addr), QState (q'_addr, v \<sigma>))"
-          
-     have st':"?st sn' = ?\<sigma>'" using sn'    
-       unfolding get_stack_def by auto     
+     let ?\<Q>' = "QStateM ((\<lambda>i. {})(q' := q'_addr), QState (q'_addr, v \<sigma>))"          
+     have st':"?st sn' = ?\<sigma>'" using sn'    unfolding get_stack_def
+       by auto     
      have v_eq:"v \<sigma> = v ?\<sigma>'" 
        by (metis a3 a4 from_nat_in_vdomain local.a1 not_access_v_f_q_eq_set st')
      then  have e_eq_v':"length (v ?\<sigma>') = 2^e \<sigma>"
        using e_eq_v by auto
      have q'_addr:"(q'_addr) \<noteq> {}" using e_gt0 q'_addr_in_new 
        unfolding new_q_addr_def by auto     
-     have "sn' \<in> (\<llangle>q\<rrangle> 1\<mapsto>\<^sub>l v)"       
+     have "sn' \<in> (\<llangle>q\<rrangle> \<mapsto>\<^sub>l v)"       
      proof-    
        have "QStateM_map (snd (snd sn')) = QStateM_map \<Q> + QStateM_map ?\<Q>'"
          using allocate_wf[of ?\<Q>', OF _ q' _ _ q'_addr_in_new e_gt0, of "(\<lambda>i. {})(q' := q'_addr)" v ?\<sigma>' set_value q, simplified, OF e_eq_v]                    
@@ -292,9 +717,9 @@ proof-
          using q'_addr unfolding plus_fun_def
          by auto       
        then have domain_q'_addr:"\<Union> (fst (get_qstate sn') ` \<llangle>q\<rrangle> (get_stack sn')) = q'_addr"
-         unfolding get_qstate_def var_exp_def 
-         using  st'  
-         unfolding get_stack_def set_value_def
+         unfolding get_qstate_def  var_exp_def 
+         using  st'  get_set[OF a3, of \<sigma> "from_nat q'"]
+         unfolding  set_value_def get_stack_def  
          by (auto simp add: get_set[OF a3] rep_nat)
        then have "Q_domain_set \<llangle>q\<rrangle> (fst (get_qstate sn')) (get_stack sn') \<noteq> {}"
          unfolding Q_domain_set_def
@@ -335,13 +760,82 @@ proof-
          ultimately show ?thesis by auto
        qed
        ultimately show ?thesis 
-         using q'_addr unfolding map_assnla_def Let_def Q_domain_set_def 
+         using q'_addr unfolding map_assnl_def Let_def Q_domain_set_def 
          by auto
      qed       
-     then have "s' \<in> Normal ` (\<llangle>q\<rrangle> 1\<mapsto>\<^sub>l v)" using sn' by auto
+     then have "s' \<in> Normal ` (\<llangle>q\<rrangle> \<mapsto>\<^sub>l v)" using sn' by auto
    } thus ?thesis unfolding valid_def by auto
+qed *)
+
+
+lemma dispose_sound:
+  assumes a0:"q \<in> variables" and  a1:"q \<in> nat_vars \<or> q \<in> nat_list_vars" and
+    a4:"n = (\<lambda>s. vec_norm (vec_of_list (v s)))" 
+  shows "\<Turnstile> ((q\<cdot>i \<mapsto>\<^sub>v v) \<and>\<^sup>* R) (Dispose q i) (( |>a\<^sub>n) \<and>\<^sup>* R)" 
+proof-
+  { fix s s'
+    let ?st = "(\<lambda>s. get_stack s) "
+    assume a00:"\<turnstile> \<langle>Dispose q i,s\<rangle> \<Rightarrow> s'" and
+            a01:"s \<in> Normal ` ((q\<cdot>i \<mapsto>\<^sub>v v) \<and>\<^sup>* R)" and
+            a02:"s' \<noteq> Fault"
+     then obtain sn where a01:"s = Normal sn" and         
+         a01a:"sn \<in>  ((q\<cdot>i \<mapsto>\<^sub>v v) \<and>\<^sup>* R)"        
+       by auto 
+     have "\<exists> \<Q>' \<Q>'' \<sigma> \<delta> . sn = (\<delta>, \<sigma>, \<Q>' + \<Q>'') \<and>
+          s' = Normal (\<delta>, \<sigma>, QStateM (QStateM_map \<Q>', vec_norm (QStateM_vector \<Q>'') \<cdot>\<^sub>q qstate \<Q>')) \<and>
+          \<Q>' ## \<Q>'' \<and> QStateM_map \<Q>'' (to_nat (get_value \<sigma> q)) \<noteq> {} \<and>
+          Q_domain (QStateM_map \<Q>'') = QStateM_map \<Q>'' (to_nat (get_value \<sigma> q))"      
+       apply (rule  QExec_Normal_elim_cases(10)[OF a00[simplified a01]])
+       using a02 by fast+
+     then obtain \<Q>' \<Q>'' \<sigma> \<delta>  where
+      f1:"sn = (\<delta>, \<sigma>, \<Q>' + \<Q>'')" and
+      f2:"s' = Normal (\<delta>, \<sigma>, QStateM (QStateM_map \<Q>', vec_norm (QStateM_vector \<Q>'') \<cdot>\<^sub>q qstate \<Q>'))" and
+      f3:"\<Q>' ## \<Q>''" and f4:"QStateM_map \<Q>'' (to_nat (get_value \<sigma> q)) \<noteq> {}" and
+      f5:"Q_domain (QStateM_map \<Q>'') = QStateM_map \<Q>'' (to_nat (get_value \<sigma> q))"       
+       by fast
+     have "QStateM_map \<Q>' = (\<lambda>s. if s \<in> QState_vars (qstate (snd (snd sn)))
+           then fst (QStateM_unfold (snd (snd sn))) s else {})" 
+       sorry
+     moreover have "vec_norm (QStateM_vector \<Q>'') \<cdot>\<^sub>q qstate \<Q>' = 
+                    qstate \<Q>' + n (fst (snd sn)) \<cdot>\<^sub>q |>"
+       sorry
+     ultimately have "QStateM (QStateM_map \<Q>', vec_norm (QStateM_vector \<Q>'') \<cdot>\<^sub>q qstate \<Q>') = 
+          ((QStateM_expr ((QState_expr q1 v2) +\<^sub>e |>\<^sub>n)) sn)"  
+       unfolding QStateM_expr_def QState_expr_def 
+          empty_state_norm_expr_def Let_def QState_plus_expr_def get_qstate_def
+          get_stack_def by auto
+     then have "(\<delta>, \<sigma>, QStateM (QStateM_map \<Q>', vec_norm (QStateM_vector \<Q>'') \<cdot>\<^sub>q qstate \<Q>')) \<in> (( |>a\<^sub>n) \<and>\<^sup>* R)"
+       using  a01d f1
+       unfolding set_qstate_def get_prob_def get_stack_def by auto
+     then have "s' \<in> Normal ` (( |>a\<^sub>n) \<and>\<^sup>* R)" using f2 by auto
+   }
+   thus ?thesis  unfolding valid_def by auto
 qed
 
+lemma dispose_sound1:
+  assumes a0:"qv = (\<lambda>s. fst (get_qstate s))" and a1:"st = get_stack" and
+    a2:"not_access_v n q" and
+    a3:"n = (\<lambda>s. vec_norm (vec_of_list (v1 s)))" and
+    a4:"P =
+    (\<llangle>q\<rrangle> 1\<mapsto>\<^sub>l v1) \<inter> (q1 1\<mapsto>\<^sub>l v2) \<inter> (\<llangle>q\<rrangle> \<inter>\<^sub>{\<^sub>} q1) \<inter>
+    {s. set_qstate s ((QStateM_expr ((QState_expr q1 v2) +\<^sub>e |>\<^sub>n)) s) \<in> Q}"
+  shows "\<Turnstile>P Dispose q {s. get_QStateM s = ((QStateM_expr ((QState_expr q1 v2) +\<^sub>e |>\<^sub>n)) s)}"
+  sorry
+
+
+(* lemma dispose_sound:
+  assumes a0:"qv = (\<lambda>s. fst (get_qstate s))" and a1:"st = get_stack" and
+    a2:"not_access_v n q" and
+    a3:"n = (\<lambda>s. vec_norm (vec_of_list (v1 s)))" and
+    a4:"P =
+    (\<llangle>q\<rrangle> 1\<mapsto>\<^sub>l v1) \<inter> (q1 1\<mapsto>\<^sub>l v2) \<inter> (\<llangle>q\<rrangle> \<inter>\<^sub>s q1) \<inter>
+    {s. get_qstate s = s1 + s2 \<and>
+        Q_domain (fst s1) = Q_domain_set \<llangle>q\<rrangle> (qv s) (st s) \<and>
+        Q_domain (fst s2) = Q_domain_set q1 (qv s) (st s) \<and>
+        set_qstate s (QStateM (fst s2, snd s2 + n (st s) \<cdot>\<^sub>q |>)) \<in> Q}"
+  shows "\<Turnstile>P Dispose q Q"
+  sorry
+*)
 
 lemma quantum_separation_logic_sound:
  "\<turnstile> P c Q \<Longrightarrow> \<Turnstile> P c Q"
